fully generic works

lexical.dfy
@@ -1,8 +1,10 @@
 include "total_order.dfy"
 	
-module Lexical_Order_Strings refines Total_Order {
+abstract module Lexical_Order refines Total_Order {
 
- 	type Element = string
+    import Entry : Total_Order
+    
+ 	type Element = seq<Entry.Element>
 
 	predicate method lte(a: Element, b: Element)
 	{
@@ -15,8 +17,8 @@ module Lexical_Order_Strings refines Total_Order {
 		if |a| == 0 && |b| == 0 then true
 		else if |a| == 0       then true
 		else if |b| == 0       then false
-		else if a[0] < b[0]    then true
-		else if a[0] > b[0]    then false
+		else if Entry.lt(a[0], b[0])    then true
+		else if Entry.lt(b[0], a[0])    then false
 		else ltedef(a[1..], b[1..])
 	}
 
@@ -26,40 +28,61 @@ module Lexical_Order_Strings refines Total_Order {
     {
     }
 
-    function method longest_common_prefix<T(==)>(a: seq<T>, b: seq<T>) : seq<T>
-        ensures longest_common_prefix<T>(a, b) <= a;
-        ensures longest_common_prefix<T>(a, b) <= b;
-        ensures
-            |longest_common_prefix<T>(a, b)| == |a| ||
-            |longest_common_prefix<T>(a, b)| == |b| ||
-            a[|longest_common_prefix<T>(a, b)|] != b[|longest_common_prefix<T>(a, b)|];
-    {
-        if |a| == 0 || |b| == 0 || a[0] != b[0] then []
-        else [a[0]] + longest_common_prefix<T>(a[1..], b[1..])
-    }
+    // function method longest_common_prefix<T(==)>(a: seq<T>, b: seq<T>) : seq<T>
+    //     ensures longest_common_prefix<T>(a, b) <= a;
+    //     ensures longest_common_prefix<T>(a, b) <= b;
+    //     ensures
+    //         |longest_common_prefix<T>(a, b)| == |a| ||
+    //         |longest_common_prefix<T>(a, b)| == |b| ||
+    //         a[|longest_common_prefix<T>(a, b)|] != b[|longest_common_prefix<T>(a, b)|];
+    // {
+    //     if |a| == 0 || |b| == 0 || a[0] != b[0] then []
+    //     else [a[0]] + longest_common_prefix<T>(a[1..], b[1..])
+    // }
 
-    lemma lexical_cmp_between_implies_common_prefix(a: string, b: string, c: string)
-        requires lte(a, b);
-        requires lte(b, c);
-        ensures
-            longest_common_prefix<char>(a, c) == longest_common_prefix<char>(a, b) ||
-            longest_common_prefix<char>(a, c) == longest_common_prefix<char>(b, c);
-    {
-        if |longest_common_prefix<char>(a, c)| > 0 {
-            assert a[0] == b[0] && b[0] == c[0];
-            lexical_cmp_between_implies_common_prefix(a[1..], b[1..], c[1..]);
-        }
-    }
+    // lemma lexical_cmp_between_implies_common_prefix(a: string, b: string, c: string)
+    //     requires lte(a, b);
+    //     requires lte(b, c);
+    //     ensures
+    //         longest_common_prefix<char>(a, c) == longest_common_prefix<char>(a, b) ||
+    //         longest_common_prefix<char>(a, c) == longest_common_prefix<char>(b, c);
+    // {
+    //     if |longest_common_prefix<char>(a, c)| > 0 {
+    //         assert a[0] == b[0] && b[0] == c[0];
+    //         lexical_cmp_between_implies_common_prefix(a[1..], b[1..], c[1..]);
+    //     }
+    // }
 
-    lemma lexical_cmp_between_implies_common_prefix_forall()
-        ensures forall a, b, c :: lte(a, b) && lte(b, c) ==>
-        longest_common_prefix<char>(a, c) == longest_common_prefix<char>(a, b) ||
-        longest_common_prefix<char>(a, c) == longest_common_prefix<char>(b, c);
-    {
-    }
+    // lemma lexical_cmp_between_implies_common_prefix_forall()
+    //     ensures forall a, b, c :: lte(a, b) && lte(b, c) ==>
+    //     longest_common_prefix<char>(a, c) == longest_common_prefix<char>(a, b) ||
+    //     longest_common_prefix<char>(a, c) == longest_common_prefix<char>(b, c);
+    // {
+    // }
 
   
 }
+
+module Seq_Int_Lex_Order refines Lexical_Order {
+    import Entry = Integer_Order
+}
+
+module Seq_Char_Lex_Order refines Lexical_Order {
+    import Entry = Char_Order
+}
+
+module String_Lex_Order refines Lexical_Order {
+    import Entry = Char_Order
+}
+
+// method Main() {
+//     print String_Lex_Order.lte("rob", "tong"); print "\n";
+//     print String_Lex_Order.lte("tong", "rob"); print "\n";
+//     print String_Lex_Order.lte("tong", "tongrob"); print "\n";
+//     print String_Lex_Order.lte("tongrob", "tong"); print "\n";
+//     print String_Lex_Order.lte("tong", "tong"); print "\n";
+//     print String_Lex_Order.lt("tong", "tong"); print "\n";
+// }
 
 // Local Variables:
 // tab-width: 4
