total_order.dfy
@@ -15,3 +15,39 @@ abstract module Total_Order {
 
 	predicate method ltedef(a: Element, b: Element)
 }
+
+module Integer_Order refines Total_Order {
+  type Element = int
+
+  predicate method lte(a: Element, b: Element) {
+    a <= b
+  }
+
+  predicate method ltedef(a: Element, b: Element) {
+    a <= b
+  }
+}
+
+module Char_Order refines Total_Order {
+  type Element = char
+
+  predicate method lte(a: Element, b: Element) {
+    a <= b
+  }
+
+  predicate method ltedef(a: Element, b: Element) {
+    a <= b
+  }
+}
+
+
+// method Main() {
+//   print Integer_Order.lt(10, 11);
+//   print "\n";
+//   print Integer_Order.lt(11, 10);
+//   print "\n";
+//   print Integer_Order.lt(11, 11);
+//   print "\n";
+//   print Integer_Order.lte(11, 11);
+//   print "\n";
+// }
